move

Veir/Data/Refinement.lean
@@ -9,23 +9,13 @@ public section
   This file defines the refinement relation from the `LLVM.Int` to `RISCV.Reg` type.
 -/
 
-open Classical in
-
-/--
-  `LLVM.Int` is refined by `RISCV.Reg`.
--/
-def IntIsRefinedByReg [DecidableEq Prop] (i : Veir.Data.LLVM.Int 64) (r : Veir.Data.RISCV.Reg) : Prop :=
-  match i with
-  | .val v => r.val = v
-  | .poison => true
-
 /--
   `LLVM.Int` is refined by `LLVM.Int`.
   `i'` refines `i` if its behaviour are a subset of the behaviours allowed by `i`.
   In particular, any concrete `i'` refines a poison `i`, but a poison `i'` does *not* refine
   any `i`.
 -/
-def IntIsRefinedByInt [DecidableEq Prop] (i i' : Veir.Data.LLVM.Int 64) : Prop :=
+def isRefinedBy (i i' : Veir.Data.LLVM.Int 64) : Prop :=
   match i with
   | .val v =>
     match i' with
